compiler/dsl/test/quark/tab.py
@@ -1,0 +1,11 @@
+#!/usr/bin/env python2.7
+
+import msg, time
+
+def main():
+  msg.init()
+  while True:
+    userinput = msg.recv()
+    msg.send('Display', userinput[1])
+
+main()
