compiler/dsl/coq/Reflex.v
@@ -17,8 +17,6 @@ Open Scope hprop_scope.
 Open Scope stsepi_scope.
 Open Scope list_scope.
 
-Axiom TODO' : False. Definition TODO {A : Type} : A := match TODO' with end.
-
 Ltac sep' := sep fail idtac.
 Ltac inv H := inversion H; subst; clear H.
 
@@ -87,7 +85,16 @@ Definition vvdesc n := vec vdesc n.
 Section WITH_PAYLOAD_DESC_VEC.
 
 Context {NB_MSG : nat}.
-Context {VVD : vvdesc NB_MSG}.
+Variable VVD : vvdesc NB_MSG.
+
+(* might as well put this here *)
+Variable COMPT : Type.
+Record comp :=
+{ comp_name : str
+; comp_cmd  : str
+; comp_args : list str
+}.
+Variable COMPS : COMPT -> comp.
 
 Definition lkup_tag (tag : fin NB_MSG) : vdesc :=
   vec_ith VVD tag.
@@ -409,14 +416,14 @@ Fixpoint expand_ktrace (kt : KTrace) : Trace :=
   | ka :: kas => expand_kaction ka ++ expand_ktrace kas
   end.
 
-Context {KST_DESC_SIZE : nat}.
-Variable KST_DESC' : vdesc' KST_DESC_SIZE.
-Definition KST_DESC_ := existT _ KST_DESC_SIZE KST_DESC'.
+Variable KSTD : vdesc.
+Notation KSTD_SIZE := (projT1 KSTD).
+Notation KSTD_DESC := (projT2 KSTD).
 
 Record kstate : Set := mkst
   { kcs : list fd
   ; ktr : [KTrace]
-  ; kst : s[[ KST_DESC_ ]]
+  ; kst : s[[ KSTD ]]
   ; kfd : list fd (* need to keep track of all the open fds... *)
   }.
 
@@ -518,20 +525,14 @@ Definition eval_op {args res} (o : op args res) : s[[ args ]] -> s[[ res ]] :=
 
 Section WITHIN_HANDLER.
 
-Variable CST : kstate.
+Variable CKST : kstate.
 Variable CFD : fd.
 Variable CMSG : msg.
 
 Let CPAY : vdesc := lkup_tag (tag CMSG).
 
-Definition payload_ith (vd : vdesc) :
-  sdenote_vdesc vd -> forall (i : fin (projT1 vd)), s[[ svec_ith (projT2 vd) i ]] :=
-  match vd as _vd with existT n pd => fun p i =>
-    shvec_ith sdenote_desc pd p i
-  end.
-
 Definition msg_param_i (i : fin (projT1 CPAY)) : s[[ svec_ith (projT2 CPAY) i ]] :=
-  payload_ith CPAY (pay CMSG) i.
+  shvec_ith _ (projT2 CPAY) (pay CMSG) i.
 
 Fixpoint all_open_payload_drop' (n : nat) :
   forall (v : vdesc' n) (drop : fd), sdenote_vdesc' n v -> hprop :=
@@ -616,13 +617,13 @@ Definition env_fds_in l (envd : vdesc) (env : s[[ envd ]]) : Prop :=
   match svec_ith (projT2 envd) i as _d return s[[ _d ]] -> Prop with
   | fd_d => fun (f : s[[ fd_d ]]) => In f l
   | _ => fun _ => True
-  end (payload_ith envd env i).
+  end (shvec_ith _ (projT2 envd) env i).
 
 Definition msg_fds_ok : Prop :=
   forall i,
   let d := svec_ith (projT2 CPAY) i in
   match d as _d return s[[ _d ]] -> Prop with
-  | fd_d => fun (f : s[[ fd_d ]]) => In f (kcs CST)
+  | fd_d => fun (f : s[[ fd_d ]]) => In f (kcs CKST)
   | _ => fun _ => True
   end (msg_param_i i).
 
@@ -631,33 +632,23 @@ Proof.
   apply forall_fin. intros i. generalize (msg_param_i i).
   destruct (svec_ith (projT2 CPAY) i).
   now left. now left.
-  intros s. destruct CST as [comps ktr]. simpl in *. apply in_dec. exact fd_eq.
+  intros s. destruct CKST as [comps ktr]. simpl in *. apply in_dec. exact fd_eq.
 Qed.
-
-(*
-Definition msg_fds_ok : hprop := all_open_payload (pay CMSG).
-
-Definition msg_fds_in : Prop := env_fds_in (components CST) CPAY (pay CMSG).
-
-Definition decide_msg_fds_in : decide msg_fds_in.
-Proof.
-  apply forall_fin. intros i. generalize (payload_ith CPAY (pay CMSG) i).
-  destruct (svec_ith (projT2 CPAY) i).
-  now left. now left.
-  intros s. destruct CST as [comps ktr]. simpl in *. apply in_dec. exact fd_eq.
-Qed.
-*)
 
 Section WITH_ENVD.
 
 Variable ENVD : vdesc.
+Notation ENVD_SIZE := (projT1 ENVD).
+Notation ENVD_DESC := (projT2 ENVD).
 
-Inductive base_expr : desc -> Set :=
-| NLit : num -> base_expr num_d
-| SLit : str -> base_expr str_d
-| Var : forall (i : fin (projT1 ENVD)), base_expr (svec_ith (projT2 ENVD) i)
-| UnOp : forall d1 d2, unop d1 d2 -> base_expr d1 -> base_expr d2
-| BinOp : forall d1 d2 d3, binop d1 d2 d3 -> base_expr d1 -> base_expr d2 -> base_expr d3
+Inductive expr : desc -> Set :=
+| SLit  : str -> expr str_d
+| NLit  : num -> expr num_d
+| Var   : forall (i : fin ENVD_SIZE), expr (svec_ith ENVD_DESC i)
+| CFd   : expr fd_d
+| StVar : forall (i : fin KSTD_SIZE), expr (svec_ith KSTD_DESC i)
+| UnOp  : forall d1 d2, unop d1 d2 -> expr d1 -> expr d2
+| BinOp : forall d1 d2 d3, binop d1 d2 d3 -> expr d1 -> expr d2 -> expr d3
 .
 
 Fixpoint payload_expr' (n : nat) (pd : vdesc' n) : Type :=
@@ -665,58 +656,30 @@ Fixpoint payload_expr' (n : nat) (pd : vdesc' n) : Type :=
   | O => fun p => unit
   | S n' => fun (pd : vdesc' (S n')) =>
     match pd with
-    | (d, pd') => base_expr d * payload_expr' n' pd'
+    | (d, pd') => expr d * payload_expr' n' pd'
     end
   end%type pd.
 
 Definition payload_expr pd := payload_expr' (projT1 pd) (projT2 pd).
 
-Inductive expr_desc :=
-| base_expr_d : desc -> expr_desc
-| msg_expr_d : expr_desc
-.
+Section WITH_PROG_ENV.
 
-Definition sdenote_expr_desc t :=
-  match t with
-  | base_expr_d d => s[[ d ]]
-  | msg_expr_d => msg
-  end.
-
-Instance SDenoted_expr_t : SDenoted expr_desc :=
-{ sdenote := sdenote_expr_desc
-}.
-
-Inductive expr : expr_desc -> Type :=
-(* an expression evaluating to one constant *)
-| MEbase : forall d, base_expr d -> expr (base_expr_d d)
-(* an expression evaluating to a vector of constants *)
-| MEmsg : forall tag, payload_expr (lkup_tag tag) -> expr msg_expr_d
-.
-
-(* Within a handler, an expression may also refer to handler-specific things *)
-Inductive hdlr_expr : expr_desc -> Type :=
-| HEexpr : forall d, expr d -> hdlr_expr d
-| HEchan : hdlr_expr (base_expr_d fd_d)
-| HEparam : forall (i : fin (projT1 CPAY)),
-  hdlr_expr (base_expr_d (svec_ith (projT2 CPAY) i))
-(* Here should be HEkst or something to access a kstate variable *)
-.
-
-Section WITH_ENV.
-
+Variable KST : s[[ KSTD ]].
 Variable ENV : s[[ ENVD ]].
 
-Fixpoint eval_base_expr (d : desc) (e : base_expr d) : s[[ d ]] :=
-  match e in base_expr _d return sdenote_desc _d with
-  | NLit n => n
-  | SLit s => s
-  | Var i => payload_ith ENVD ENV i
+Fixpoint eval_expr (d : desc) (e : expr d) : s[[ d ]] :=
+  match e in expr _d return sdenote_desc _d with
+  | SLit s  => s
+  | NLit n  => n
+  | Var i   => shvec_ith _ (projT2 ENVD) ENV i
+  | CFd     => CFD
+  | StVar i => shvec_ith _ (projT2 KSTD) KST i
   | UnOp t1 t2 op e =>
-    let v := eval_base_expr t1 e in
+    let v := eval_expr t1 e in
     eval_unop op v
   | BinOp t1 t2 t3 op e1 e2 =>
-    let v1 := eval_base_expr t1 e1 in
-    let v2 := eval_base_expr t2 e2 in
+    let v1 := eval_expr t1 e1 in
+    let v2 := eval_expr t2 e2 in
     eval_binop op v1 v2
   end.
 
@@ -731,74 +694,200 @@ Fixpoint eval_payload_expr' (n : nat) :
     let (d, pd') as _pd return res (S n') _pd := pd in
     fun e =>
       let (v, e') := e in
-      (eval_base_expr d v, eval_payload_expr' n' pd' e')
+      (eval_expr d v, eval_payload_expr' n' pd' e')
   end.
 
 Definition eval_payload_expr (pd : vdesc) (e : payload_expr pd) : s[[ pd ]] :=
   eval_payload_expr' (projT1 pd) (projT2 pd) e.
 
-Definition eval_expr (d : expr_desc) (e : expr d) : s[[ d ]] :=
-  match e with
-  | MEbase d' e' => eval_base_expr d' e'
-  | MEmsg t pl =>
-    let p := eval_payload_expr (lkup_tag t) pl in
-    {| tag := t; pay := p |}
-  end.
-
-Definition eval_hdlr_expr (d : expr_desc) (e : hdlr_expr d) : s[[ d ]] :=
-  match e with
-  | HEexpr d' e' => eval_expr d' e'
-  | HEchan => CFD
-  | HEparam i => msg_param_i i
-  end.
-
-Inductive cmd (e : expr_desc -> Type) : Type :=
-| Send : e (base_expr_d fd_d) -> expr msg_expr_d -> cmd e
-| STChange : forall i, e (base_expr_d (svec_ith (projT2 KST_DESC_) i)) -> cmd e
+Inductive cmd : Type :=
+| Send  : expr fd_d -> forall (t : fin NB_MSG), payload_expr (lkup_tag t) -> cmd
+| Spawn : COMPT -> forall (i : fin ENVD_SIZE), svec_ith ENVD_DESC i = fd_d -> cmd
+| StUpd : forall i, svec_ith (projT2 KSTD) i <> fd_d -> expr (svec_ith (projT2 KSTD) i) -> cmd
 .
 
-Definition init_cmd := cmd expr.
+(*
+Inductive base_expr : desc -> Set :=
+| SLit  : str -> base_expr str_d
+| NLit  : num -> base_expr num_d
+| Var   : forall (i : fin ENVD_SIZE), base_expr (svec_ith ENVD_DESC i)
+.
 
-Definition init_prog := list init_cmd.
+Inductive hdlr_expr : desc -> Set :=
+| Base  : forall d, base_expr d -> hdlr_expr d
+| CFd   : hdlr_expr fd_d
+| StVar : forall (i : fin KSTD_SIZE), hdlr_expr (svec_ith KSTD_DESC i)
+.
 
-Definition hdlr_cmd := cmd hdlr_expr.
+Section WITH_EXPR.
 
-Definition hdlr_prog := list hdlr_cmd.
+Variable EXPR : desc -> Set.
 
-End WITH_ENV.
+Inductive expr : desc -> Set :=
+| NoOp  : forall d, EXPR d -> expr d
+| UnOp  : forall d1 d2, unop d1 d2 -> expr d1 -> expr d2
+| BinOp : forall d1 d2 d3, binop d1 d2 d3 -> expr d1 -> expr d2 -> expr d3
+.
+
+Fixpoint payload_expr' (n : nat) (pd : vdesc' n) : Type :=
+  match n as _n return vdesc' _n -> Type with
+  | O => fun p => unit
+  | S n' => fun (pd : vdesc' (S n')) =>
+    match pd with
+    | (d, pd') => expr d * payload_expr' n' pd'
+    end
+  end%type pd.
+
+Definition payload_expr pd := payload_expr' (projT1 pd) (projT2 pd).
+
+End WITH_EXPR.
+
+Section WITH_PROG_ENV.
+
+Variable ENV : s[[ ENVD ]].
+
+Fixpoint eval_base_expr (d : desc) (e : base_expr d) : s[[ d ]] :=
+  match e in base_expr _d return sdenote_desc _d with
+  | SLit s => s
+  | NLit n => n
+  | Var i  => payload_ith ENVD ENV i
+  end.
+
+Fixpoint eval_hdlr_expr (d : desc) (e : hdlr_expr d) : s[[ d ]] :=
+  match e in hdlr_expr _d return sdenote_desc _d with
+  | Base d b  => eval_base_expr d b
+  | CFd     => CFD
+  | StVar i => payload_ith KSTD (kst KST) i
+  end.
+
+Section WITH_EVAL_EXPR.
+
+Variable EXPR : desc -> Set.
+Variable EVAL_EXPR : forall (d : desc) (e : EXPR d), s[[ d ]].
+
+Fixpoint eval_expr (d : desc) (e : expr EXPR d) : s[[ d ]] :=
+  match e in expr _ _d return sdenote_desc _d with
+  | NoOp d e => EVAL_EXPR d e
+  | UnOp t1 t2 op e =>
+    let v := eval_expr t1 e in
+    eval_unop op v
+  | BinOp t1 t2 t3 op e1 e2 =>
+    let v1 := eval_expr t1 e1 in
+    let v2 := eval_expr t2 e2 in
+    eval_binop op v1 v2
+  end.
+
+Fixpoint eval_payload_expr' (n : nat) :
+  forall (pd : vdesc' n), payload_expr' EXPR n pd -> s[[ pd ]] :=
+  let res n pd := payload_expr' EXPR n pd -> s[[ pd ]] in
+  match n as _n return
+    forall (pd : vdesc' _n), res _n pd
+  with
+  | O => fun _ _ => tt
+  | S n' => fun pd =>
+    let (d, pd') as _pd return res (S n') _pd := pd in
+    fun e =>
+      let (v, e') := e in
+      (eval_expr d v, eval_payload_expr' n' pd' e')
+  end.
+
+Definition eval_payload_expr (pd : vdesc) (e : payload_expr EXPR pd) : s[[ pd ]] :=
+  eval_payload_expr' (projT1 pd) (projT2 pd) e.
+
+Inductive cmd : Type :=
+| Send  : expr EXPR fd_d -> forall (t : fin NB_MSG), payload_expr EXPR (lkup_tag t) -> cmd
+| Spawn : COMPT -> cmd
+| StUpd : forall i, expr EXPR (svec_ith (projT2 KSTD) i) -> cmd
+.
+
+*)
 
 Record init_state :=
 { init_comps : list fd
 ; init_ktr   : [KTrace]%type
 ; init_env   : s[[ ENVD ]]
-; init_kst   : s[[ KST_DESC_ ]]
+; init_kst   : s[[ KSTD ]]
 }.
 
-Definition init_state_run_cmd (s : init_state) : init_cmd -> init_state :=
-  let (cs, tr, e, st) := s in
-  fun c =>
-    match c with
-    | Send fe me =>
-      let f := eval_expr e _ fe in
-      let m := eval_expr e _ me in
-      {| init_comps := cs
-       ; init_ktr   := tr ~~~ KSend f m :: tr
-       ; init_env   := e
-       ; init_kst   := st
-      |}
-    | STChange i ve =>
-      let v := eval_expr e _ ve in
-      {| init_comps := cs
-       ; init_ktr   := tr
-       ; init_env   := e
-       ; init_kst   := shvec_replace_ith sdenote_desc (projT2 KST_DESC_) st i v
-      |}
-    end.
+Definition init_cmd := init_state -> cmd.
 
-Fixpoint init_state_run_prog (s : init_state) (p : init_prog) : init_state :=
+Definition init_prog := list init_cmd.
+
+Definition hdlr_cmd := kstate -> cmd.
+
+Definition hdlr_prog := kstate -> list hdlr_cmd.
+
+End WITH_PROG_ENV.
+
+Definition cmd_input_desc (c : cmd)  :=
+  match c with
+  | Send _ _ _  => None
+  | Spawn _ _ _ => Some fd_d
+  | StUpd _ _ _ => None
+  end.
+
+Definition sdenote_option {T : Type} (sdenote_content : T -> Set) (o : option T) : Set :=
+  match o with
+  | Some x => sdenote_content x
+  | None => unit
+  end.
+
+Definition cmd_input (c : cmd) : Set :=
+  sdenote_option sdenote_desc (cmd_input_desc c).
+
+Definition shvec_replace_cast {d} {i : fin ENVD_SIZE} (EQ : svec_ith ENVD_DESC i = d) e v
+  :=
+  shvec_replace_ith sdenote_desc _ e i
+    (match EQ in _ = _d return s[[ _d ]] -> _ with Logic.eq_refl => fun x => x end v).
+
+Definition init_state_run_cmd (s : init_state) (cmd : cmd) : cmd_input cmd -> init_state :=
+  let (cs, tr, e, st) := s in
+  match cmd as _cmd return cmd_input _cmd -> init_state with
+
+  | Send fe t me => fun _ =>
+    let f := eval_expr st e _ fe in
+    let m := eval_payload_expr st e _ me in
+    {| init_comps := cs
+     ; init_ktr   := tr ~~~ KSend f (Build_msg t m) :: tr
+     ; init_env   := e
+     ; init_kst   := st
+     |}
+
+  | Spawn ct i EQ => fun c =>
+    let comp := COMPS ct in
+    {| init_comps := c :: cs
+     ; init_ktr   := tr ~~~ KExec (comp_cmd comp) (comp_args comp) c :: tr
+     ; init_env   := shvec_replace_cast EQ e c
+     ; init_kst   := st
+     |}
+
+  | StUpd i _ ve => fun _ =>
+    let v := eval_expr st e _ ve in
+    {| init_comps := cs
+     ; init_ktr   := tr
+     ; init_env   := e
+     ; init_kst   := shvec_replace_ith _ _ st i v
+     |}
+  end.
+
+Fixpoint init_state_run_prog_return_type s p :=
   match p with
-  | c :: cs => init_state_run_prog (init_state_run_cmd s c) cs
-  | nil => s
+  | c :: cs =>
+    sigT (fun (x : cmd_input (c s)) =>
+            init_state_run_prog_return_type (init_state_run_cmd s (c s) x) cs)
+  | nil => unit
+  end.
+
+Fixpoint init_state_run_prog (s : init_state) (p : init_prog) :
+  init_state_run_prog_return_type s p -> init_state
+  :=
+  match p as _p return init_state_run_prog_return_type s _p -> init_state with
+  | c :: cs => fun v =>
+    match v with
+    | existT x rest =>
+      init_state_run_prog (init_state_run_cmd s (c s) x) cs rest
+    end
+  | nil => fun _ => s
   end.
 
 Record hdlr_state :=
@@ -807,41 +896,67 @@ Record hdlr_state :=
 }.
 
 (* This should probably move out once the environment can change *)
-Definition hdlr_state_run_cmd (s : hdlr_state) : hdlr_cmd -> hdlr_state :=
+Definition hdlr_state_run_cmd (s : hdlr_state) (cmd : cmd) : cmd_input cmd -> hdlr_state :=
   let (s', env) := s in
   let (cs, tr, st, fd) := s' in
-  fun c =>
-    match c with
-    | Send fe me =>
-      let f := eval_hdlr_expr env _ fe in
-      let m := eval_expr env _ me in
-      {| hdlr_kst :=
-           {| kcs := cs
-            ; ktr := tr ~~~ KSend f m :: tr
-            ; kst := st
-            ; kfd := fd
-            |}
-       ; hdlr_env := env
-      |}
-    | STChange i ve =>
-      let v := eval_hdlr_expr env _ ve in
-      {| hdlr_kst :=
-           {| kcs := cs
-            ; ktr := tr
-            ; kst := shvec_replace_ith sdenote_desc (projT2 KST_DESC_) st i v
-            ; kfd := fd
-            |}
-       ; hdlr_env := env
-      |}
-    end.
+  match cmd with
 
-Fixpoint hdlr_state_run_prog (s : hdlr_state) (p : hdlr_prog) : hdlr_state :=
-  match p with
-  | nil => s
-  | c::cs => hdlr_state_run_prog (hdlr_state_run_cmd s c) cs
+  | Send fe t me => fun _ =>
+    let f := eval_expr st env _ fe in
+    let m := eval_payload_expr st env _ me in
+    {| hdlr_kst :=
+         {| kcs := cs
+          ; ktr := tr ~~~ KSend f (Build_msg t m) :: tr
+          ; kst := st
+          ; kfd := fd
+          |}
+     ; hdlr_env := env
+    |}
+
+  | Spawn ct i EQ => fun c =>
+    let comp := COMPS ct in
+    {| hdlr_kst :=
+         {| kcs := c :: cs
+          ; ktr := tr ~~~ KExec (comp_cmd comp) (comp_args comp) c :: tr
+          ; kst := st
+          ; kfd := fd
+          |}
+     ; hdlr_env := shvec_replace_cast EQ env c
+     |}
+
+  | StUpd i _ ve => fun _ =>
+    let v := eval_expr st env _ ve in
+    {| hdlr_kst :=
+         {| kcs := cs
+          ; ktr := tr
+          ; kst := shvec_replace_ith _ _ st i v
+          ; kfd := fd
+          |}
+     ; hdlr_env := env
+     |}
   end.
 
-Axiom devnull : fd.
+Fixpoint hdlr_state_run_prog_return_type s p :=
+  match p with
+  | c :: cs =>
+    sigT (fun (x : cmd_input (c (hdlr_kst s))) =>
+            hdlr_state_run_prog_return_type (hdlr_state_run_cmd s (c (hdlr_kst s)) x) cs)
+  | nil => unit
+  end.
+
+Fixpoint hdlr_state_run_prog (s : hdlr_state) (p : list hdlr_cmd) :
+  hdlr_state_run_prog_return_type s p -> hdlr_state
+  :=
+  match p as _p return hdlr_state_run_prog_return_type s _p -> hdlr_state with
+  | c :: cs => fun v =>
+    match v with
+    | existT x rest =>
+      hdlr_state_run_prog (hdlr_state_run_cmd s (c (hdlr_kst s)) x) cs rest
+    end
+  | nil => fun _ => s
+  end.
+
+Definition devnull := Num "000" "000".
 
 Axiom devnull_open : emp ==> open devnull.
 
@@ -864,30 +979,35 @@ Fixpoint default_payload' (n : nat) :
 Definition default_payload (v : vdesc) : s[[ v ]] :=
   default_payload' (projT1 v) (projT2 v).
 
-Fixpoint kstate_run_prog (s : kstate) (p : hdlr_prog) : kstate :=
-  let hs :=
-    {| hdlr_kst := s
-     ; hdlr_env := default_payload ENVD
-     |} in
-  hdlr_kst (hdlr_state_run_prog hs p).
+Definition default_hdlr_state s :=
+  {| hdlr_kst := s; hdlr_env := default_payload ENVD |}.
+
+Definition kstate_run_prog_return_type s p :=
+  hdlr_state_run_prog_return_type (default_hdlr_state s) p.
+
+Definition kstate_run_prog (s : kstate) (p : hdlr_prog)
+  (input : kstate_run_prog_return_type s (p s))
+  : kstate :=
+  hdlr_kst (hdlr_state_run_prog (default_hdlr_state s) (p s) input).
 
 End WITH_ENVD.
+
 End WITHIN_HANDLER.
 
-Variable INIT_ENVD : vdesc.
-Variable INIT_PROG : init_prog INIT_ENVD.
+Variable IENVD : vdesc.
+Variable IPROG : init_prog IENVD.
 
 Definition initial_init_state :=
   {| init_comps := nil
    ; init_ktr   := [nil]%inhabited
-   ; init_env   := default_payload INIT_ENVD
-   ; init_kst   := default_payload KST_DESC_
+   ; init_env   := default_payload IENVD
+   ; init_kst   := default_payload KSTD
    |}.
 
 Section WITH_HANDLER.
 
-Definition handlers := forall (m : msg) (f : fd) (s : kstate),
-                         sigT (fun (vd : vdesc) => hdlr_prog m vd).
+Definition handlers := forall (m : msg) (cfd : fd),
+  sigT (fun (prog_envd : vdesc) => hdlr_prog prog_envd).
 
 Variable HANDLERS : handlers.
 
@@ -912,15 +1032,15 @@ Definition payload_fds (v : vdesc) : s[[ v ]] -> list fd :=
 
 Inductive Reach : kstate -> Prop :=
 | Reach_init :
-  forall s,
-  s = init_state_run_prog INIT_ENVD initial_init_state INIT_PROG ->
+  forall s input,
+  s = init_state_run_prog devnull IENVD initial_init_state IPROG input ->
   Reach {| kcs := init_comps _ s
          ; ktr := init_ktr _ s
          ; kst := init_kst _ s
-         ; kfd := payload_fds _ (init_env _ s)
+         ; kfd := payload_fds _ (init_kst _ s) ++ payload_fds _ (init_env _ s)
          |}
 | Reach_valid :
-  forall s f m tr s' s'',
+  forall s f m tr s' s'' input,
   msg_fds_ok s m ->
   let cs := kcs s in
   ktr s = [tr]%inhabited ->
@@ -930,7 +1050,7 @@ Inductive Reach : kstate -> Prop :=
         ; kst := kst s
         ; kfd := kfd s
         |} ->
-  s'' = kstate_run_prog f m (projT1 (HANDLERS m f s')) s' (projT2 (HANDLERS m f s')) ->
+  s'' = kstate_run_prog f (projT1 (HANDLERS m f)) s' (projT2 (HANDLERS m f)) input ->
   Reach {| kcs := kcs s''
          ; ktr := ktr s''
          ; kst := kst s''
@@ -959,9 +1079,9 @@ Inductive Reach : kstate -> Prop :=
      ; kfd := kfd s
      |}
 .
-(*
+
 Definition kstate_inv s : hprop :=
-  tr :~~ ktr s in emp
+  tr :~~ ktr s in open devnull
   * traced (expand_ktrace tr) * [Reach s]
   * all_open (kcs s) * all_open (kfd s)
   .
@@ -1028,8 +1148,8 @@ Ltac uninhabit :=
   | [ H1 : ktr ?s = [_]%inhabited, H2 : ktr ?s = [_]%inhabited |- _ ] =>
     rewrite H1 in H2; apply pack_injective in H2;
     rewrite -> H2 in * || rewrite <- H2 in * (* subst may be blocked *)
-  | [ H : [_]%inhabited = [_]%inhabited |- _ ] =>
-    apply pack_injective in H; subst
+  | [ H : [?x]%inhabited = [?y]%inhabited |- _ ] =>
+    apply pack_injective in H; try first [subst x | subst y]
   end.
 
 Ltac misc :=
@@ -1050,73 +1170,124 @@ Ltac sep'' :=
   sep unfoldr simplr.
 
 Lemma eval_base_expr_fd :
-  forall l d envd e v env,
+  forall l cfd d envd e v env st,
+  In cfd l ->
   env_fds_in l envd env ->
-  eval_base_expr envd env d e = v ->
+  env_fds_in l _ st ->
+  eval_expr cfd envd st env d e = v ->
   match d as _d return (s[[ _d ]] -> Prop) with
   | fd_d => fun f => In f l
   | _ => fun _ => True
   end v.
 Proof.
-  induction e; try tauto; intros vd env OK E; simpl in *.
-  subst. exact (OK i).
+  induction e; try tauto; intros vd env st IN OKE OKS E; simpl in *.
+  subst. exact (OKE i).
+  now subst.
+  subst. exact (OKS i).
   now destruct u.
   now destruct b.
 Qed.
 
-Lemma eval_expr_fd :
-  forall l d envd e v env,
-  env_fds_in l envd env ->
-  eval_expr envd env d e = v ->
-  match d as _d return (sdenote_expr_desc _d -> Prop) with
-  | base_expr_d fd_d => fun f => In f l
+Theorem eval_expr_fd_in_payload : forall cfd envd e d fe v st,
+  eval_expr cfd envd st e d fe = v ->
+  match d as _d return sdenote_desc _d -> Prop with
+  | fd_d => fun f => f = cfd \/ fd_in_payload f envd e \/ fd_in_payload f KSTD st
   | _ => fun _ => True
   end v.
 Proof.
-  intros l d envd. induction e; intros vd env OK E; simpl in *.
-  destruct b; try tauto; simpl in *.
-  subst. exact (OK i).
-  now destruct u.
-  now destruct b1.
-  exact I.
-Qed.
-
-Theorem eval_expr_fd_in_payload : forall envd d fe v s,
-  eval_expr envd (init_env envd s) d fe = v ->
-  match d as _d return sdenote_expr_desc _d -> Prop with
-  | base_expr_d fd_d => fun f => fd_in_payload f envd (init_env envd s)
-  | _ => fun _ => True
-  end v.
-Proof.
-  intros envd d.
-  destruct fe; intros v s E; intuition simpl in *.
-  destruct b as []_eqn; intuition simpl in *. subst.
+  intros cfd envd e d.
+  destruct fe; intros v st E; simpl in *; try tauto.
   pose proof (
     shvec_ith_in sdenote_desc desc_eqdec UIP_refl_desc (projT2 envd)
-    (init_env envd s) i
+    e i
   ).
   destruct envd as [n envd]. simpl in *.
-  unfold payload_ith.
-  generalize dependent (
-    shvec_ith sdenote_desc envd
-      (init_env (existT (fun n0 : nat => vdesc' n0) n envd) s) i
-  ).
+  generalize dependent (shvec_ith sdenote_desc envd e i).
   intros.
-  destruct (svec_ith envd i); tauto.
+  destruct (svec_ith envd i); try tauto.
+  subst. right. left. exact H.
+  now left.
+  pose proof (
+    shvec_ith_in sdenote_desc desc_eqdec UIP_refl_desc (projT2 KSTD)
+    st i
+  ).
+  destruct envd as [n envd].
+  rewrite E in H. clear E.
+  generalize dependent (svec_ith KSTD_DESC i).
+  intros. destruct d; tauto.
   now destruct u.
-  now destruct b0.
+  now destruct b.
 Qed.
 
 Definition init_invariant {envd} (s : init_state envd) :=
-  all_open (init_comps _ s)
-  * all_open_payload (init_env _ s).
+  open devnull * all_open (init_comps _ s)
+  * all_open_payload (init_env _ s) * all_open_payload (init_kst _ s).
+
+Definition open_payload_frame {EXPR envd fed} (fe : expr EXPR fed) (f : s[[ fed ]])
+  (cfd : fd) (env : s[[ envd ]]) (st : s[[ KSTD ]])
+  : hprop
+  :=
+  match fe in expr _ _d return s[[ _d ]] -> hprop with
+  | SLit s => fun _ => emp
+  | NLit n => fun _ => emp
+  | Var i => fun f =>
+    match svec_ith (projT2 EXPR) i as _s return s[[ _s ]] -> hprop with
+    | num_d => fun _ => emp
+    | str_d => fun _ => emp
+    | fd_d  => fun f => open cfd * all_open_payload_drop f env * all_open_payload st
+    end f
+  | CFd => fun _ => all_open_payload env * all_open_payload st
+  | StVar i => fun f =>
+    match svec_ith KSTD_DESC i as _s return s[[ _s ]] -> hprop with
+    | num_d => fun _ => emp
+    | str_d => fun _ => emp
+    | fd_d  => fun f => open cfd * all_open_payload env * all_open_payload_drop f st
+    end f
+  | UnOp d1 d2 op e1 => fun _ => emp
+  | BinOp d1 d2 d3 op e1 e2 => fun _ => emp
+  end f.
+
+(*
+Definition open_payload_frame {envd} (cfd : fd) (f : fd) (pl : s[[ envd ]]) :=
+  if fd_eq f cfd
+  then all_open_payload pl
+  else open cfd * all_open_payload_drop f pl
+.
+*)
+
+Theorem numd_neq_fdd : num_d = fd_d -> False. Proof. discriminate. Qed.
+Theorem strd_neq_fdd : str_d = fd_d -> False. Proof. discriminate. Qed.
+
+Theorem all_open_payload_replace' :
+  forall (ds : nat) (d : vdesc' ds) (st : sdenote_vdesc' ds d) i v
+         (H : svec_ith d i = fd_d -> False),
+  all_open_payload' _ _ st ==>
+  all_open_payload' _ _ (shvec_replace_ith sdenote_desc d st i v).
+Proof.
+  intros. induction ds.
+  destruct i.
+  simpl in d, i, st.
+  destruct d as [d d']. destruct i as [i'|]. destruct st as [st st'].
+  specialize (IHds d' st' i' v H).
+  simpl. destruct d; sep''.
+  simpl in *. destruct d, st; simpl in *; sep''.
+Qed.
+
+Theorem all_open_payload_replace :
+  forall (d : vdesc) (st : sdenote_vdesc d) i v (H : svec_ith (projT2 d) i = fd_d -> False),
+  all_open_payload st ==>
+  all_open_payload (shvec_replace_ith sdenote_desc (projT2 d) st i v).
+Proof.
+  intros. now apply all_open_payload_replace'.
+Qed.
 
 Definition run_init_cmd :
-  forall (envd : vdesc) (s : init_state envd) (c : init_cmd envd),
-  STsep (tr :~~ init_ktr envd s in
+  forall (prog_envd : vdesc) (s : init_state prog_envd) (c : cmd prog_envd),
+  STsep (tr :~~ init_ktr prog_envd s in
           init_invariant s * traced (expand_ktrace tr))
-        (fun s' : init_state envd => tr :~~ init_ktr envd s' in
-          init_invariant s' * traced (expand_ktrace tr) * [s' = init_state_run_cmd envd s c]).
+        (fun s' : init_state prog_envd => tr :~~ init_ktr prog_envd s' in
+          init_invariant s' * traced (expand_ktrace tr) *
+          [exists input, s' = init_state_run_cmd devnull prog_envd s c input]).
 Proof.
   intros; refine (
     let cs := init_comps _ s in
@@ -1124,84 +1295,348 @@ Proof.
     let e  := init_env _ s in
     let st := init_kst _ s in
     match c with
-    | Send fe me =>
+
+    | Send fe t me =>
       (* /!\ We lose track of the let-open equalities if existentials remain,
          make sure that Coq can infer _all_ the underscores. *)
-      let f := eval_expr _ e _ fe in
-      let m := eval_expr _ e _ me in
-      send_msg f m (tr ~~~ expand_ktrace tr)
-      <@> all_open cs * all_open_payload_drop f e;;
+      let f := eval_expr devnull _ st e _ fe in
+      let m := eval_payload_expr devnull _ st e _ me in
+      send_msg f (Build_msg t m) (tr ~~~ expand_ktrace tr)
+      <@> all_open cs * open_payload_frame fe f devnull e st;;
 
-      let tr := tr ~~~ KSend f m :: tr in
+      let tr := tr ~~~ KSend f (Build_msg t m) :: tr in
       {{ Return {| init_comps := cs
                  ; init_ktr   := tr
                  ; init_env   := e
                  ; init_kst   := st
                  |} }}
+
+    | Spawn ct i EQ =>
+      let c_cmd := comp_cmd (COMPS ct) in
+      let c_args := comp_args (COMPS ct) in
+      c <- exec c_cmd c_args (tr ~~~ expand_ktrace tr)
+        <@> open devnull * all_open (init_comps prog_envd s)
+          * all_open_payload (init_env prog_envd s)
+          * all_open_payload (init_kst prog_envd s);
+
+      let tr := tr ~~~ KExec c_cmd c_args c :: tr in
+      {{ Return {| init_comps := c :: cs
+                 ; init_ktr   := tr
+                 ; init_env   := shvec_replace_cast _ EQ e c
+                 ; init_kst   := st
+                 |} }}
+
+    | StUpd i _ ve =>
+      let v := eval_expr devnull _ st e _ ve in
+      {{ Return {| init_comps := cs
+                 ; init_ktr   := tr
+                 ; init_env   := e
+                 ; init_kst   := shvec_replace_ith _ _ st i v
+                 |} }}      
+
     end
-  ); unfold init_invariant, cs, e; sep''.
-  pose proof eval_expr_fd_in_payload as E.
-  specialize (E _ _ fe f s (Logic.eq_refl f)). now simpl in E.
-  pose proof eval_expr_fd_in_payload as E.
-  specialize (E _ _ fe f s (Logic.eq_refl f)). now simpl in E.
+  );
+  unfold init_invariant, cs, e, open_payload_frame, cmd_input; sep''.
+
+  unfold f. clear f.
+  refine (
+    match fe as _fe in expr _ _d return (
+      _d = fd_d ->
+      all_open_payload (init_kst prog_envd s) *
+      (all_open_payload (init_env prog_envd s) * open devnull) ==>
+      match _d as __d return s[[ __d ]] -> hprop with
+      | num_d => fun _ => emp
+      | str_d => fun _ => emp
+      | fd_d  => fun f => open f
+      end (eval_expr devnull prog_envd st e _d _fe)
+      *
+      match _fe in expr _ __d return (sdenote_desc __d -> hprop) with
+      | SLit _ => fun _ => emp
+      | NLit _ => fun _ => emp
+      | Var i =>
+        fun f : sdenote_desc (svec_ith (projT2 prog_envd) i) =>
+        match svec_ith (projT2 prog_envd) i as _s return (sdenote_desc _s -> hprop) with
+        | num_d => fun _ => emp
+        | str_d => fun _ => emp
+        | fd_d =>
+          fun f0 : fd =>
+            open devnull * all_open_payload_drop f0 (init_env prog_envd s) *
+            all_open_payload st
+        end f
+      | CFd =>
+        fun _ =>
+          all_open_payload (init_env prog_envd s) * all_open_payload st
+      | StVar i =>
+        fun f : sdenote_desc (svec_ith KSTD_DESC i) =>
+          match svec_ith KSTD_DESC i as _s return (sdenote_desc _s -> hprop) with
+            | num_d => fun _ : num => emp
+            | str_d => fun _ : str => emp
+            | fd_d =>
+              fun f0 : fd =>
+           open devnull * all_open_payload (init_env prog_envd s) *
+           all_open_payload_drop f0 st
+          end f
+      | UnOp _ d2 _ _ => fun _ => emp
+      | BinOp _ _ d3 _ _ _ => fun _ => emp
+      end (eval_expr devnull prog_envd st e _d _fe)
+    ) with
+    | NLit _ => fun bad => match numd_neq_fdd bad with end
+    | SLit _ => fun bad => match strd_neq_fdd bad with end
+    | _      => fun _   => _
+    end (Logic.eq_refl fd_d)
+  ).
+  simpl.
+
+  assert (
+    match svec_ith (projT2 prog_envd) i as _x return s[[ _x ]] -> Prop with
+    | num_d => fun _ => True
+    | str_d => fun _ => True
+    | fd_d  => fun v => fd_in_payload v prog_envd (init_env prog_envd s)
+    end (shvec_ith sdenote_desc (projT2 prog_envd) e i)
+  ).
+  pose proof (shvec_ith_in) as IN.
+  specialize (
+    IN desc sdenote_desc desc_eqdec UIP_refl_desc (projT1 prog_envd) (projT2 prog_envd) e i
+  ).
+  generalize dependent (shvec_ith sdenote_desc (projT2 prog_envd) e i).
+  destruct (svec_ith (projT2 prog_envd) i); tauto.
+
+  revert H0.
+
+  refine (
+    match svec_ith (projT2 prog_envd) i as _x return (
+      _x = fd_d -> forall (v : s[[ _x ]]),
+   match _x as __x return (s[[ __x ]] -> Prop)
+   with
+   | num_d => fun _ => True
+   | str_d => fun _ => True
+   | fd_d  => fun v => fd_in_payload v prog_envd (init_env prog_envd s)
+   end v ->
+   all_open_payload (init_kst prog_envd s) *
+   (all_open_payload (init_env prog_envd s) * open devnull) ==>
+   match _x as __d return (s[[__d]] -> hprop) with
+   | num_d => fun _ : s[[num_d]] => emp
+   | str_d => fun _ : s[[str_d]] => emp
+   | fd_d => fun f : s[[fd_d]] => open f
+   end v *
+   match _x as _s return (sdenote_desc _s -> hprop)
+   with
+   | num_d => fun _ : sdenote_desc num_d => emp
+   | str_d => fun _ : sdenote_desc str_d => emp
+   | fd_d =>
+       fun f0 : fd =>
+       open devnull * all_open_payload_drop f0 (init_env prog_envd s) *
+       all_open_payload st
+   end v
+    ) with
+    | num_d => fun bad => match numd_neq_fdd bad with end
+    | str_d => fun bad => match strd_neq_fdd bad with end
+    | fd_d  => fun _ => _
+    end _H (shvec_ith sdenote_desc (projT2 prog_envd) e i)
+  ).
+
+  intros. sep''.
+  sep''.
+  sep''.
+  
+  assert (
+    match svec_ith KSTD_DESC i as _x return s[[ _x ]] -> Prop with
+    | num_d => fun _ => True
+    | str_d => fun _ => True
+    | fd_d  => fun v =>
+      fd_in_payload v KSTD st
+    end (shvec_ith sdenote_desc KSTD_DESC st i)
+  ).
+  pose proof (shvec_ith_in) as IN.
+  specialize (
+    IN desc sdenote_desc desc_eqdec UIP_refl_desc KSTD_SIZE KSTD_DESC st i
+  ).
+  generalize dependent (shvec_ith sdenote_desc KSTD_DESC st i).
+  destruct (svec_ith KSTD_DESC i); tauto.
+
+  generalize dependent (
+    shvec_ith sdenote_desc KSTD_DESC st i
+  ).
+  destruct (svec_ith KSTD_DESC i); try discriminate.
+  intros. sep''.
+
+  destruct u; discriminate.
+  destruct b; discriminate.
+
+  unfold f. clear f.
+  refine (
+    match fe as _fe in expr _ _d return (
+      _d = fd_d ->
+      match _d as __d return s[[ __d ]] -> hprop with
+      | num_d => fun _ => emp
+      | str_d => fun _ => emp
+      | fd_d  => fun f => open f
+      end (eval_expr devnull prog_envd st e _d _fe)
+      *
+   match _fe in expr _ __d return (sdenote_desc __d -> hprop) with
+   | SLit _ => fun _ : str => emp
+   | NLit _ => fun _ : num => emp
+   | Var i =>
+       fun f : sdenote_desc (svec_ith (projT2 prog_envd) i) =>
+       match svec_ith (projT2 prog_envd) i as _s return (sdenote_desc _s -> hprop)
+       with
+       | num_d => fun _ : num => emp
+       | str_d => fun _ : str => emp
+       | fd_d =>
+           fun f0 : fd =>
+           open devnull * all_open_payload_drop f0 (init_env prog_envd s) *
+           all_open_payload st
+       end f
+   | CFd =>
+       fun _ : fd =>
+       all_open_payload (init_env prog_envd s) * all_open_payload st
+   | StVar i =>
+       fun f : sdenote_desc (svec_ith KSTD_DESC i) =>
+       match svec_ith KSTD_DESC i as _s return (sdenote_desc _s -> hprop) with
+       | num_d => fun _ : num => emp
+       | str_d => fun _ : str => emp
+       | fd_d =>
+           fun f0 : fd =>
+           open devnull * all_open_payload (init_env prog_envd s) *
+           all_open_payload_drop f0 st
+       end f
+   | UnOp _ d2 _ _ => fun _ : sdenote_desc d2 => emp
+   | BinOp _ _ d3 _ _ _ => fun _ : sdenote_desc d3 => emp
+   end (eval_expr devnull prog_envd st e _d _fe) ==>
+   all_open_payload st *
+   (all_open_payload (init_env prog_envd s) * open devnull) *
+   [exists input : unit,
+      {|
+      init_comps := init_comps prog_envd s;
+      init_ktr := [KSend (eval_expr devnull prog_envd st e fd_d fe)
+                     {| tag := t; pay := m |} :: x0];
+      init_env := init_env prog_envd s;
+      init_kst := st |} =
+      init_state_run_cmd devnull prog_envd s (Send prog_envd fe t me) input]
+
+    ) with
+    | NLit _ => fun bad => match numd_neq_fdd bad with end
+    | SLit _ => fun bad => match strd_neq_fdd bad with end
+    | _      => fun _   => _
+    end (Logic.eq_refl fd_d)
+  ).
+  simpl.
+
+  assert (
+    match svec_ith (projT2 prog_envd) i as _x return s[[ _x ]] -> Prop with
+    | num_d => fun _ => True
+    | str_d => fun _ => True
+    | fd_d  => fun v => fd_in_payload v prog_envd (init_env prog_envd s)
+    end (shvec_ith sdenote_desc (projT2 prog_envd) e i)
+  ).
+  pose proof (shvec_ith_in) as IN.
+  specialize (
+    IN desc sdenote_desc desc_eqdec UIP_refl_desc (projT1 prog_envd) (projT2 prog_envd) e i
+  ).
+  generalize dependent (shvec_ith sdenote_desc (projT2 prog_envd) e i).
+  destruct (svec_ith (projT2 prog_envd) i); tauto.
+
+  revert H.
+
+  refine (
+    match svec_ith (projT2 prog_envd) i as _x return (
+      _x = fd_d -> forall (v : s[[ _x ]]),
+
+   match _x as __x return (s[[ __x ]] -> Prop) with
+   | num_d => fun _ : s[[num_d]] => True
+   | str_d => fun _ : s[[str_d]] => True
+   | fd_d =>
+       fun v : s[[fd_d]] => fd_in_payload v prog_envd (init_env prog_envd s)
+   end v ->
+   match _x as __d return (sdenote_desc __d -> hprop) with
+   | num_d => fun _ : num => emp
+   | str_d => fun _ : str => emp
+   | fd_d => fun f : fd => open f
+   end v *
+   match _x as _s return (sdenote_desc _s -> hprop) with
+   | num_d => fun _ : num => emp
+   | str_d => fun _ : str => emp
+   | fd_d =>
+       fun f0 : fd =>
+       open devnull * all_open_payload_drop f0 (init_env prog_envd s) *
+       all_open_payload st
+   end v ==>
+   all_open_payload st *
+   (all_open_payload (init_env prog_envd s) * open devnull) *
+   [exists input : unit,
+      {|
+      init_comps := init_comps prog_envd s;
+      init_ktr := [KSend (eval_expr devnull prog_envd st e fd_d fe)
+                     {| tag := t; pay := m |} :: x0];
+      init_env := init_env prog_envd s;
+      init_kst := st |} =
+      init_state_run_cmd devnull prog_envd s (Send prog_envd fe t me) input]
+
+    ) with
+    | num_d => fun bad => match numd_neq_fdd bad with end
+    | str_d => fun bad => match strd_neq_fdd bad with end
+    | fd_d  => fun _ => _
+    end _H (shvec_ith sdenote_desc (projT2 prog_envd) e i)
+  ).
+
+  intros. sep''. apply himp_pure'. exists tt.
+  unfold init_state_run_cmd. unfold m, e in *. destruct s. simpl in *. sep''.
+
+  sep''.
   apply himp_pure'.
-  unfold init_state_run_cmd. destruct s. simpl.
-  sep''. unfold f, m, e. simpl in *. sep''.
+  exists tt.
+  unfold init_state_run_cmd. unfold m, e in *. destruct s. simpl in *. sep''.
+  admit.
+  destruct u; discriminate.
+  destruct b; discriminate.
+  isolate (
+    all_open_payload (init_env prog_envd s) ==>
+    all_open_payload (shvec_replace_cast prog_envd EQ (init_env prog_envd s) c0)
+  ).
+  admit.
+  apply himp_pure'. exists c0. destruct s. simpl in *. sep''.
+  isolate (
+    all_open_payload (init_kst prog_envd s) ==>
+    all_open_payload (shvec_replace_ith sdenote_desc KSTD_DESC st i v)
+  ).
+  now apply all_open_payload_replace.
+  apply himp_pure'. exists tt. destruct s. sep''.
   (* dirty proof, could be made nicer... *)
 Qed.
-
-(* that seems wrong and unneeded
-Fixpoint init_env_fds_ok' (n : nat) : forall (v : vdesc' n), sdenote_vdesc' n v -> hprop.
-Proof.
-  destruct n as [|n']. exact (fun _ _ => emp).
-  intros v. destruct v as [d v']. destruct d.
-  intros vv. destruct vv as (vd, vv'). exact (init_env_fds_ok' n' v' vv').
-  intros vv. destruct vv as (vd, vv'). exact (init_env_fds_ok' n' v' vv').
-  intros vv. destruct vv as (vd, vv'). exact (open vd * init_env_fds_ok' n' v' vv').
-Qed.
-
-(* is this needed? *)
-Fixpoint init_env_fds_ok'' (n : nat) :
-  forall (v : vdesc' n), sdenote_vdesc' n v -> hprop :=
-  match n with
-  | 0 => fun _ _ => emp
-  | S n0 =>
-    fun v =>
-    let (d, v') as p return (sdenote_vdesc' (S n0) p -> hprop) := v in
-    fun vv =>
-    let (vd, _) := vv in
-    match d as d0 return (s[[d0]] -> hprop) with
-    | fd_d => fun vd => open vd
-    | _ => fun _ => emp
-    end vd
-  end
-.
-*)
 
 Definition run_init_prog :
   forall (envd : vdesc) (s : init_state envd) (p : init_prog envd),
   STsep (tr :~~ init_ktr envd s in
           init_invariant s * traced (expand_ktrace tr))
         (fun s' : init_state envd => tr :~~ init_ktr envd s' in
-          init_invariant s' * traced (expand_ktrace tr) * [s' = init_state_run_prog envd s p]).
+          init_invariant s' * traced (expand_ktrace tr)
+          * [exists input, s' = init_state_run_prog devnull envd s p input]).
 Proof.
   intros; refine (
     Fix2
       (fun p s => tr :~~ init_ktr envd s in
         init_invariant s * traced (expand_ktrace tr))
       (fun p s (s' : init_state envd) => tr :~~ init_ktr envd s' in
-        init_invariant s' * traced (expand_ktrace tr) * [s' = init_state_run_prog envd s p])
+        init_invariant s' * traced (expand_ktrace tr)
+        * [exists input, s' = init_state_run_prog devnull envd s p input])
       (fun self p s =>
         match p with
         | nil => {{ Return s }}
         | c::cs =>
-          s' <- run_init_cmd envd s c;
-          s'' <- self cs s' <@> [s' = init_state_run_cmd envd s c];
+          s' <- run_init_cmd envd s (c s);
+          s'' <- self cs s' <@> [exists input, s' = init_state_run_cmd devnull envd s (c s) input];
           {{ Return s'' }}
         end
       )
     p s
   ); sep''.
+  apply himp_pure'. exists tt. reflexivity.
+  apply himp_pure'. destruct H1 as [h1 H1]. destruct H2 as [h2 H2]. subst s'.
+  exists (existT 
+            (fun x : cmd_input envd (c s0) =>
+               init_state_run_prog_return_type devnull envd
+                 (init_state_run_cmd devnull envd s0 (c s0) x) cs)
+            h2 h1). exact H1.
 Qed.
 
 Theorem all_open_default_payload : forall henv,
@@ -1221,6 +1656,14 @@ Qed.
 Axiom all_open_payload_to_all_open : forall v p,
   all_open_payload p ==> all_open (payload_fds v p).
 
+Theorem all_open_concat : forall a b,
+  all_open a * all_open b ==> all_open (a ++ b).
+Proof.
+  induction a.
+  simpl. sep'.
+  simpl. sep'.
+Qed.
+
 Definition kinit :
   forall (_ : unit),
   STsep (traced nil)
@@ -1228,54 +1671,34 @@ Definition kinit :
 Proof.
   intros; refine (
     let s := initial_init_state in
-    s' <- run_init_prog _ s INIT_PROG;
+    s' <- run_init_prog _ s IPROG;
     {{ Return {| kcs := init_comps _ s'
                ; ktr := init_ktr _ s'
                ; kst := init_kst _ s'
-               ; kfd := nil ++ payload_fds _ (init_env _ s')
+               ; kfd := nil ++ payload_fds KSTD (init_kst IENVD s')
+                            ++ payload_fds IENVD (init_env IENVD s')
                |}
      }}
   ); unfold init_invariant; sep''.
+  isolate (emp ==> open devnull). apply devnull_open.
+  isolate (emp ==> all_open_payload (default_payload IENVD)).
   apply all_open_default_payload.
+  apply all_open_default_payload.
+  isolate (
+    all_open_payload (init_kst IENVD s') *
+    all_open_payload (init_env IENVD s') ==>
+    all_open (payload_fds KSTD (init_kst IENVD s')
+                          ++ payload_fds IENVD (init_env IENVD s'))
+  ).
+  eapply himp_trans; [ | apply all_open_concat ].
+  apply himp_split.
   apply all_open_payload_to_all_open.
+  apply all_open_payload_to_all_open.
+  apply himp_pure'. destruct H2 as [h2 H2]. sep''.
 Qed.
-
-(*
-Definition run_init_cmd :
-  forall (envd : vdesc) (s : init_state envd) (c : init_cmd envd),
-  STsep (tr :~~ init_ktr envd s in
-          init_invariant s * traced (expand_ktrace tr))
-        (fun s' : init_state envd => tr :~~ init_ktr envd s' in
-          init_invariant s' * traced (expand_ktrace tr) * [s' = init_state_run_cmd envd s c]).
-*)
 
 Definition env_fds_ok envd (hs : hdlr_state envd) :=
   env_fds_in (kfd (hdlr_kst envd hs)) envd (hdlr_env envd hs).
-
-Theorem eval_hdlr_expr_fd_in : forall cfd cm envd d fe v (s : hdlr_state envd),
-  let (kst, env) := s in
-  env_fds_ok envd s ->
-  msg_fds_ok kst cm ->
-  In cfd (kcs kst) ->
-  eval_hdlr_expr cfd cm envd env d fe = v ->
-  match d as _d return sdenote_expr_desc _d -> Prop with
-  | base_expr_d fd_d => fun f => In f (kcs kst) \/ In f (kfd kst)
-  | _ => fun _ => True
-  end v.
-Proof.
-  intros until s. destruct s as [kst env]. simpl. intros F M I E. subst.
-  destruct fe; simpl in *; try tauto.
-  destruct e; simpl in *; try tauto.
-  destruct b; simpl in *; try tauto.
-  specialize (F i). simpl in F.
-  generalize dependent (payload_ith envd env i).
-  destruct (svec_ith (projT2 envd) i); tauto.
-  now destruct u.
-  now destruct b1.
-  specialize (M i). simpl in *.
-  generalize dependent (msg_param_i cm i).
-  destruct (svec_ith (projT2 (lkup_tag (tag cm))) i); tauto.
-Qed.
 
 Definition hdlr_invariant {envd} (cfd : fd) (cm : msg) (s : hdlr_state envd) :=
   let (kst, env) := s in
@@ -1284,55 +1707,135 @@ Definition hdlr_invariant {envd} (cfd : fd) (cm : msg) (s : hdlr_state envd) :=
   * [In cfd (kcs kst)] * [msg_fds_ok kst cm] * [env_fds_ok envd s]
 .
 
+Lemma env_fds_in_app_r : forall envd env a b,
+  env_fds_in a envd env ->
+  env_fds_in (b ++ a) envd env.
+Proof.
+  intros. induction b. now simpl. simpl. unfold env_fds_in in *.
+  intros i. specialize (IHb i). clear H.
+  generalize dependent (shvec_ith sdenote_desc (projT2 envd) env i).
+  destruct (svec_ith (projT2 envd) i); try tauto.
+  intros. now right.
+Qed.
+
 Definition run_hdlr_cmd :
-  forall (cfd : fd) (cm : msg) (envd : vdesc) (s : hdlr_state envd) (c : hdlr_cmd cm envd),
+  forall (cfd : fd) (cm : msg) (envd : vdesc) (s : hdlr_state envd) (c : cmd envd),
   STsep (tr :~~ ktr (hdlr_kst _ s) in
           hdlr_invariant cfd cm s * traced (expand_ktrace tr))
         (fun s' : hdlr_state envd => tr :~~ ktr (hdlr_kst _ s') in
           hdlr_invariant cfd cm s' * traced (expand_ktrace tr)
-          * [s' = hdlr_state_run_cmd cfd cm envd s c]).
+          * [exists input, s' = hdlr_state_run_cmd cfd envd s c input]).
 Proof.
   intros; refine (
-    (* you lose the equations if you try to let (st, env, fds) := s *)
-    let st := hdlr_kst _ s in
-    let env := hdlr_env _ s in
-    let comps := kcs st in
-    let tr := ktr st in
-    let fds := kfd st in
-    match c with
-    | Send fe me =>
-      let f := eval_hdlr_expr cfd cm _ env _ fe in
-      let m := eval_expr envd env _ me in
-      send_msg f m
-      (tr ~~~ expand_ktrace tr)
-      <@> all_open_drop (comps ++ fds) f * all_open_payload (pay cm)
-      * [In cfd comps] * [msg_fds_ok st cm] * [env_fds_ok envd s];;
+  (* you lose the equations if you try to let (st, env, fds) := s *)
+  let st := hdlr_kst _ s in
+  let env := hdlr_env _ s in
+  let cs := kcs st in
+  let tr := ktr st in
+  let fds := kfd st in
+  match c with
 
-      let tr := tr ~~~ KSend f m :: tr in
-      {{Return {| hdlr_kst := {| kcs := comps ; ktr := tr ; kst := kst st ; kfd := fds |}
-                ; hdlr_env := env
-                |}
-      }}
-    end
-  ); unfold env, fds, hdlr_invariant in *; clear env fds; sep fail idtac;
-  pose proof (eval_hdlr_expr_fd_in cfd cm _ _ fe f s) as E;
-  destruct s as (kst, env).
+  | Send fe t me =>
+    let f := eval_expr cfd _ (kst st) env _ fe in
+    let m := eval_payload_expr cfd envd (kst st) env _ me in
+    send_msg f (Build_msg t m)
+    (tr ~~~ expand_ktrace tr)
+    <@> all_open_drop (cs ++ fds) f * all_open_payload (pay cm)
+      * [In cfd cs] * [msg_fds_ok st cm] * [env_fds_ok envd s];;
+
+    let tr := tr ~~~ KSend f (Build_msg t m) :: tr in
+    {{Return {| hdlr_kst := {| kcs := cs ; ktr := tr ; kst := kst st ; kfd := fds |}
+              ; hdlr_env := env
+              |}
+    }}
+
+  | Spawn ct i EQ =>
+    let c_cmd := comp_cmd (COMPS ct) in
+    let c_args := comp_args (COMPS ct) in
+    c <- exec c_cmd c_args (tr ~~~ expand_ktrace tr)
+      <@> all_open (cs ++ fds) * all_open_payload (pay cm)
+        * [In cfd cs] * [msg_fds_ok st cm] * [env_fds_ok envd s];
+
+    let tr := tr ~~~ KExec c_cmd c_args c :: tr in
+    {{ Return {| hdlr_kst := {| kcs := c :: cs
+                              ; ktr := tr
+                              ; kst := kst st
+                              ; kfd := fds |}
+               ; hdlr_env := shvec_replace_cast _ EQ env c
+               |}
+    }}
+
+  | StUpd i _ ve =>
+    let v := eval_expr cfd _ (kst st) env _ ve in
+    {{ Return {| hdlr_kst := {| kcs := cs
+                              ; ktr := tr
+                              ; kst := shvec_replace_ith _ _ (kst st) i v
+                              ; kfd := fds
+                              |}
+               ; hdlr_env := env
+               |}
+    }}
+
+  end
+  ); unfold env, fds, hdlr_invariant, cmd_input in *; clear env fds; sep fail idtac;
+  destruct s as (kst, env);
   sep''.
-  sep''.
-  apply himp_pure'. destruct kst as (kcs, ktr, kst, kfd). simpl in *.
-  unfold comps in *. clear comps. sep''.
-  apply himp_pure'. destruct kst as (cs, ktr, kst, kfd). simpl in *.
-  unfold comps in *. clear comps. sep''.
+
+  pose proof (
+    eval_expr_fd_in_payload cfd envd
+                            (hdlr_env _ {| hdlr_kst := kst; hdlr_env := env |})
+                            _ fe f _ (Logic.eq_refl f)
+  ) as E. simpl in E. intuition.
+  rewrite H0. apply in_or_app. now left.
+  unfold env_fds_ok in H4. simpl in H4. unfold env_fds_in in H4.
+  unfold fd_in_payload, fd_in_payload' in H1.
+  pose proof shvec_in_ith as I.
+  specialize (I _ _ _ _ _ _ _ _ H1).
+  destruct I as [i [e I] ]. specialize (H4 i).
+  generalize dependent (shvec_ith sdenote_desc (projT2 envd) env i).
+  rewrite <- e. intros. apply in_or_app. subst. now right.
+  admit. (* TODO *)
+
+  pose proof (
+    eval_expr_fd_in_payload cfd envd
+                            (hdlr_env _ {| hdlr_kst := kst; hdlr_env := env |})
+                            _ fe f _ (Logic.eq_refl f)
+  ) as E. simpl in E. intuition.
+  rewrite H. apply in_or_app. now left.
+  unfold env_fds_ok in H5. simpl in H5. unfold env_fds_in in H5.
+  unfold fd_in_payload, fd_in_payload' in H1.
+  pose proof shvec_in_ith as I.
+  specialize (I _ _ _ _ _ _ _ _ H1).
+  destruct I as [i [e I] ]. specialize (H5 i).
+  generalize dependent (shvec_ith sdenote_desc (projT2 envd) env i).
+  rewrite <- e. intros. apply in_or_app. subst. now right.
+  admit. (* TODO *)
+
+  apply himp_pure'. exists tt. destruct kst. simpl in *. sep''.
+
+  (* this could go in a tactic *)
+  
+  apply himp_trans with (Q := emp * emp * emp). sep''. repeat apply himp_split; apply himp_pure'.
+
+  admit. (* TODO *)
+
+  unfold msg_fds_ok. simpl. intros i0. specialize (H4 i0). simpl in H4.
+  generalize dependent (msg_param_i cm i0). intros.
+  destruct (svec_ith (projT2 (lkup_tag (tag cm))) i0); try tauto.
+
+  exists c0. destruct kst; simpl in *. sep''.
+  destruct kst. apply himp_pure'. exists tt. sep''.
   (* so ugly... *)
 Qed.
 
 Definition run_hdlr_prog :
-  forall (cfd : fd) (cm : msg) (envd : vdesc) (s : hdlr_state envd) (p : hdlr_prog cm envd),
+  forall (cfd : fd) (cm : msg) (envd : vdesc) (s : hdlr_state envd) (p : hdlr_prog envd),
   STsep (tr :~~ ktr (hdlr_kst _ s) in
           hdlr_invariant cfd cm s * traced (expand_ktrace tr))
         (fun s' : hdlr_state envd => tr :~~ ktr (hdlr_kst _ s') in
           hdlr_invariant cfd cm s' * traced (expand_ktrace tr)
-          * [s' = hdlr_state_run_prog cfd cm envd s p]).
+          * [exists input, s' =
+               hdlr_state_run_prog cfd envd s (p (hdlr_kst _ s)) input]).
 Proof.
   intros; refine (
     Fix2
@@ -1342,27 +1845,28 @@ Proof.
       (fun p s (s' : hdlr_state envd) =>
         tr :~~ ktr (hdlr_kst _ s') in
           hdlr_invariant cfd cm s' * traced (expand_ktrace tr)
-          * [s' = hdlr_state_run_prog cfd cm envd s p])
+                                            (* TODO: this works but seems wrong *)
+          * [exists input, s' = hdlr_state_run_prog cfd envd s p input])
       (fun self p s =>
         match p with
         | nil =>
           {{ Return s }}
         | c::cs =>
-          s' <- run_hdlr_cmd cfd cm envd s c;
-          s'' <- self cs s' <@> [hdlr_state_run_cmd cfd cm envd s c = s'];
+          s' <- run_hdlr_cmd cfd cm envd s (c (hdlr_kst _ s));
+          s'' <- self cs s'
+          <@> [exists input, s' = hdlr_state_run_cmd cfd envd s (c (hdlr_kst _ s)) input];
           {{ Return s'' }}
         end)
-    p s
+    (p (hdlr_kst _ s)) s
   );
   sep''.
-Qed.
-
-Theorem all_open_concat : forall a b,
-  all_open a * all_open b ==> all_open (a ++ b).
-Proof.
-  induction a.
-  simpl. sep'.
-  simpl. sep'.
+  apply himp_pure'. now exists tt.
+  apply himp_pure'. destruct H1 as [h1 H1]. destruct H2 as [h2 H2]. subst s'.
+  exists (existT 
+            (fun x : cmd_input envd (c (hdlr_kst envd s0)) =>
+               hdlr_state_run_prog_return_type cfd envd
+                 (hdlr_state_run_cmd cfd envd s0 (c (hdlr_kst envd s0)) x) cs)
+            h2 h1). exact H1.
 Qed.
 
 Theorem all_open_unconcat : forall a b,
@@ -1374,9 +1878,9 @@ Proof.
 Qed.
 
 Axiom in_devnull_default_payload: forall henv l,
-  env_fds_in (devnull :: l) henv (default_payload henv).*)
+  env_fds_in (devnull :: l) henv (default_payload henv).
 
-(*Definition kbody:
+Definition kbody:
   forall s,
   STsep (kstate_inv s)
         (fun s' => kstate_inv s').
@@ -1389,12 +1893,12 @@ Proof.
     let fd := kfd s in
     c <- select cs
     (tr ~~~ expand_ktrace tr)
-    <@> (tr ~~ [Reach s] * all_open cs * all_open fd);
+    <@> (tr ~~ [Reach s] * open devnull * all_open cs * all_open fd);
 
     let tr := tr ~~~ KSelect cs c :: tr in
     mm <- recv_msg c
     (tr ~~~ expand_ktrace tr)
-    <@> (tr ~~ [In c cs] * [Reach s] * all_open_drop cs c * all_open fd);
+    <@> (tr ~~ [In c cs] * [Reach s] * open devnull * all_open_drop cs c * all_open fd);
 
     match mm with
     | inl m =>
@@ -1402,8 +1906,8 @@ Proof.
       let ck := msg_fds_ck s m in
       match ck as ck' return ck = ck' -> _ with
       | left _ => fun _ =>
-        let henv  := projT1 (HANDLERS m) in
-        let hprog := projT2 (HANDLERS m) in
+        let henv  := projT1 (HANDLERS m c) in
+        let hprog := projT2 (HANDLERS m c) in
         let s' := {| hdlr_kst := {| kcs := cs
                                   ; ktr := tr
                                   ; kst := st
@@ -1411,7 +1915,7 @@ Proof.
                    ; hdlr_env := default_payload henv
                    |}
         in
-        s'' <- run_hdlr_prog c m henv s' hprog <@> [Reach s];
+        s'' <- run_hdlr_prog c m henv s' hprog <@> [Reach s] * open devnull;
         (* we need to add the payload open fds to kfd so as not to keep track of any
            linear resource *)
         let s''' := {| hdlr_kst := {| kcs := kcs (hdlr_kst _ s'')
@@ -1432,8 +1936,8 @@ Proof.
   ); unfold hdlr_invariant in *; sep''.
 
   isolate (
-    all_open_drop cs c * open c * all_open fd
-    ==> all_open (cs ++ (*devnull ::*) fd)
+    open c * all_open_drop cs c * all_open fd
+    ==> all_open (cs ++ fd)
   ).
 
   apply himp_trans with (Q := all_open cs * all_open fd); sep''.
@@ -1441,8 +1945,7 @@ Proof.
   sep''. (*apply devnull_open.*) apply all_open_concat.
   apply himp_pure'. unfold env_fds_ok. simpl. admit. (*apply in_devnull_default_payload.*)
 
-  destruct (hdlr_state_run_prog c m henv s' hprog) as [kst'' env'']_eqn.
-  simpl in *. sep''.
+  destruct s'' as [kst'' ?]; simpl in *; sep''.
   isolate (
     all_open (kcs kst'' ++ kfd kst'') * all_open_payload (pay m)
     ==> all_open (kcs kst'') * all_open (kfd kst'' ++ payload_fds _ (pay m))
@@ -1455,22 +1958,15 @@ Proof.
   apply all_open_payload_to_all_open.
   apply all_open_concat.
 
-  sep''. constructor; auto.
-  eapply Reach_valid with (s := s) (s' := (hdlr_kst _ s')); eauto.
-  unfold s'. simpl. unfold cs, st, fd. sep''.
-
+  apply himp_pure'. destruct H4 as [input H4].
+  destruct (ktr s) as []_eqn. simpl in *.
+  apply pack_injective in H1. subst x1.
+  eapply Reach_valid with (f := c) (s := s) (s' := (hdlr_kst _ s')) (input := input); eauto.
   unfold kstate_run_prog. simpl.
-  unfold s' in Heqh.
-  unfold henv, hprog in Heqh. rewrite Heqh. now simpl.
+  apply f_equal with (f := hdlr_kst _) in H4. simpl in H4. rewrite H4. f_equal.
 
-  isolate (
-    all_open_payload (pay m) * all_open fd ==>
-    all_open (fd ++ payload_fds (lkup_tag (tag m)) (pay m))
-  ).
   eapply himp_trans; [ | apply all_open_concat ]. sep''.
   apply all_open_payload_to_all_open.
-
-  sep''.
 Qed.
 
 Definition kloop:
@@ -1503,21 +1999,46 @@ Proof.
     {{ Return sN }}
   );
   sep'.
-Qed.*)
+Qed.
 
 End WITH_HANDLER.
 
 End WITH_PAYLOAD_DESC_VEC.
 
-(*Record spec :=
-{ NB_MSG    : nat
-; PAY_DESC  : vvdesc NB_MSG
-; INIT_ENVD : vdesc
-; INIT      : @init_prog NB_MSG PAY_DESC INIT_ENVD
-; KST_DESC  : vdesc
-; HANDLERS  : handlers (VVD := PAY_DESC)
+Record spec :=
+{ NB_MSG   : nat
+; PAYD     : vvdesc NB_MSG
+; IENVD    : vdesc
+; KSTD     : vdesc
+; COMPT    : Type
+; COMPS    : COMPT -> comp
+; INIT     : init_prog PAYD COMPT KSTD IENVD
+; HANDLERS : handlers PAYD COMPT KSTD
 }.
 
 Definition mk_main (s : spec) :=
-  @main _ (PAY_DESC s) _ (projT2 (KST_DESC s)) _ (INIT s) (HANDLERS s).
-*)
+  @main _ (PAYD s) (COMPT s) (COMPS s) (KSTD s) (IENVD s) (INIT s) (HANDLERS s).
+
+Fixpoint mk_vdesc' l : vdesc' (List.length l) :=
+  match l with
+  | nil     => tt
+  | x :: xs => (x, mk_vdesc' xs)
+  end.
+
+Definition mk_vdesc l : vdesc := existT _ (List.length l) (mk_vdesc' l).
+
+Fixpoint mk_vvdesc (l : list (string * list desc)) : vvdesc (List.length l) :=
+  match l with
+  | nil          => tt
+  | (_, x) :: xs => (mk_vdesc x, mk_vvdesc xs)
+  end.
+
+Definition mk_comp name cmd args :=
+  {| comp_name := str_of_string name
+   ; comp_cmd  := str_of_string cmd
+   ; comp_args := List.map str_of_string args
+   |}.
+
+Notation " [ ] " := nil.
+Notation " [ x ] " := (cons x nil).
+Notation " [ x ; .. ; y ] " := (cons x .. (cons y nil) ..).
