compiler/pollang/ReflexKState.v
@@ -5,64 +5,70 @@ Require Import ReflexBase.
 Require Import ReflexDenoted.
 Require Import ReflexVec.
 Require Import ReflexHVec.
+Require Import ReflexFin.
+
+Open Scope string_scope.
 
 Definition NB_MSG : nat := 2.
 
-Definition PAY_DESC : vvdesc NB_MSG :=
-  ( existT _ 1 (str_d, tt) (*User name payload.*)
-   , ( existT _ 2 (str_d, (num_d, tt)) (*Auth response from system payload.*)
-    , tt)
-  ).
-
-Definition INIT_ENVD : vdesc := existT _ 0 tt.
-
-Definition KST_DESC_SIZE := 2.
+Definition PAYD : vvdesc NB_MSG :=
+  mk_vvdesc
+  [ ("User", [str_d]) (*User name payload.*)
+   ; ("Auth", [str_d; num_d]) (*Auth response from system payload.*)
+  ].
 
 (*State is (username, authres)*)
-Definition KST_DESC : vdesc' KST_DESC_SIZE := (str_d, (num_d, tt)).
+Definition KSTD : vdesc := mk_vdesc [str_d; num_d].
+Definition st_user : fin (projT1 KSTD) := None.
+Definition st_authed : fin (projT1 KSTD) := Some None.
 
-Definition INIT : @init_prog NB_MSG PAY_DESC _ KST_DESC INIT_ENVD :=
-  nil.
+Notation msg_user := (None) (only parsing).
+Notation msg_authed := (Some None) (only parsing).
 
-Definition HANDLERS : handlers (VVD := PAY_DESC) KST_DESC :=
-  (fun m f st =>
-    match tag m as _tm return
-      @sdenote _ SDenoted_vdesc (lkup_tag (VVD := PAY_DESC) _tm) -> _
+Definition IENVD : vdesc := mk_vdesc [].
+
+Inductive COMPT : Type := Stupid.
+
+Definition COMPS (t : COMPT) : comp :=
+  match t with
+  | Stupid => mk_comp "Echo" "test/echo-00/test.py" []
+  end.
+
+Definition INIT : init_prog PAYD COMPT KSTD IENVD := [].
+
+Definition HANDLERS : handlers PAYD COMPT KSTD :=
+  (fun m cfd =>
+    match tag PAYD m as _tm return
+      @sdenote _ SDenoted_vdesc (lkup_tag PAYD _tm) -> _
     with
-    | None => fun pl =>
-       let (u, _) := pl in
+    | msg_user => fun pl =>
        let envd := existT _ 0 tt in
-       if num_eq (@shvec_ith _ _ _
-                                (KST_DESC:svec desc KST_DESC_SIZE)
-                                (kst _ st) (Some None))
-                    (num_of_nat 0)
-       then existT _ envd (nil) (*Ignore.*)
-       else if str_eq (@shvec_ith _ _ _
-                                (KST_DESC:svec desc KST_DESC_SIZE)
-                                (kst _ st) None)
-                    u
-            then existT _ envd (
-                          let (u, _) := pl in
-                          Send _ _ _
-                               (HEchan _ _)
-                               (@MEmsg _ PAY_DESC envd None (SLit _ u, tt))
-                               :: nil
-                          )
-            else existT _ envd (nil) (*Ignore.*)
-    | Some None => fun pl =>
+       existT (fun d => hdlr_prog PAYD COMPT KSTD d) envd (
+         let (u, _) := pl in fun st =>
+           if num_eq (@shvec_ith _ _ (projT1 KSTD)
+                                 (projT2 KSTD)
+                                 (kst _ _ st) st_authed)
+                                 (num_of_nat 0)
+           then [] (*Ignore.*)
+           else if str_eq (@shvec_ith _ _ (projT1 KSTD)
+                                      (projT2 KSTD)
+                                      (kst _ _ st) st_user)
+                                      u
+                then [ fun s => Send PAYD _ _ _ (CFd _ _) None (SLit _ _ u, tt) ]
+                else [] (*Ignore.*)
+              )
+    | msg_authed => fun pl =>
        let envd := existT _ 0 tt in
-       existT _ envd (
+       existT (fun d => hdlr_prog PAYD COMPT KSTD d) envd (
         let (u, pl') := pl in
-        let (res, _) := pl' in
-        STChange KST_DESC _ _
-          None (HEexpr _ _ _ (MEbase _ _ (SLit _ u)))
-        :: STChange KST_DESC _ _
-             (Some None) (HEexpr _ _ _ (MEbase _ _ (NLit _ res)))
-        :: nil
+        let (res, _) := pl' in fun st =>
+        [ fun _ => StUpd _ _ KSTD _ st_user strd_neq_fdd  (SLit _ _ u)
+        ; fun _ => StUpd _ _ KSTD _ st_authed numd_neq_fdd (NLit _ _ res)
+        ]
       )
     | Some (Some bad) => fun _ =>
       match bad with end
-    end (pay m)
+    end (pay _ m)
   ).
 
 Require Import PolLang.
@@ -71,13 +77,13 @@ Require Import Tactics.
 Require Import Ynot.
 
 Theorem release : forall st tr u,
-  Reach _ _ INIT HANDLERS st -> ktr _ st = inhabits tr ->
-  Release NB_MSG PAY_DESC
-          (@KORecv NB_MSG PAY_DESC None
-                   (Some (@Build_opt_msg NB_MSG PAY_DESC
+  Reach _ _ COMPS _ _ INIT HANDLERS st -> ktr _ _ st = inhabits tr ->
+  Release NB_MSG PAYD
+          (@KORecv NB_MSG PAYD None
+                   (Some (@Build_opt_msg NB_MSG PAYD
                                          (Some None) (Some u, (None, tt)))))
-          (@KOSend NB_MSG PAY_DESC None
-                   (Some (@Build_opt_msg NB_MSG PAY_DESC
+          (@KOSend NB_MSG PAYD None
+                   (Some (@Build_opt_msg NB_MSG PAYD
                                          None (Some u, tt))))
           tr.
 Proof.
