compiler/dsl/coq/ReflexQuark.v
@@ -1,0 +1,105 @@
+Require Import String.
+
+Require Import Reflex.
+Require Import ReflexBase.
+Require Import ReflexDenoted.
+Require Import ReflexFin.
+Require Import ReflexHVec.
+Require Import ReflexVec.
+
+Open Scope string_scope.
+
+Definition NB_MSG : nat := 3.
+
+Definition PAYD : vvdesc NB_MSG := mk_vvdesc
+  [ ("Input",   [str_d])
+  ; ("Display", [str_d])
+  ; ("Quit",    [ ])
+  ].
+
+Notation Input   := (None) (only parsing).
+Notation Display := (Some None) (only parsing).
+Notation Quit    := (Some (Some None)) (only parsing).
+
+Definition KSTD : vdesc := mk_vdesc
+  [ fd_d (* curtab *)
+  ; fd_d (* screen *)
+  ; fd_d (* user-input *)
+  ].
+
+Notation curtab    := (None) (only parsing).
+Notation screen    := (Some None) (only parsing).
+Notation userinput := (Some (Some None)) (only parsing).
+
+Definition IENVD : vdesc := mk_vdesc
+  [ fd_d (* curtab *)
+  ; fd_d (* screen *)
+  ; fd_d (* userinput *)
+  ].
+
+Notation v_t := (None) (only parsing).
+Notation v_s := (Some None) (only parsing).
+Notation v_u := (Some (Some None)) (only parsing).
+
+Inductive COMPT : Type := Tab | Screen | UserInput.
+
+Definition COMPS (t : COMPT) : comp :=
+  match t with
+  | Tab       => mk_comp "Tab"       "test/quark/tab.py"        []
+  | Screen    => mk_comp "Screen"    "test/quark/screen.py"     []
+  | UserInput => mk_comp "UserInput" "test/quark/user-input.py" []
+  end.
+
+Definition INIT : init_prog PAYD COMPT KSTD IENVD :=
+  [ fun s => Spawn _ _ _ IENVD Tab       v_t (Logic.eq_refl _)
+  ; fun s => Spawn _ _ _ IENVD Screen    v_s (Logic.eq_refl _)
+  ; fun s => Spawn _ _ _ IENVD UserInput v_u (Logic.eq_refl _)
+  ].
+
+Definition HANDLERS : handlers PAYD COMPT KSTD :=
+  (fun m cfd =>
+    match tag PAYD m as _tm return
+      @sdenote _ SDenoted_vdesc (lkup_tag PAYD _tm) -> _
+    with
+
+    | Input => fun pl =>
+       let envd := mk_vdesc [] in
+       existT (fun d => hdlr_prog PAYD COMPT KSTD d) envd (
+         let (input, _) := pl in fun st0 =>
+         if fd_eq cfd (shvec_ith (n := projT1 KSTD) _ (projT2 KSTD) (kst _ _ st0) userinput)
+         then
+           [ fun s => Send PAYD COMPT KSTD envd (StVar KSTD _ curtab) Input (SLit _ _ input, tt) ]
+         else
+           []
+       )
+
+    | Display => fun pl =>
+       let envd := mk_vdesc [] in
+       existT (fun d => hdlr_prog PAYD COMPT KSTD d) envd (
+         let (url, _) := pl in fun st0 =>
+         if fd_eq cfd (shvec_ith (n := projT1 KSTD) _ (projT2 KSTD) (kst _ _ st0) curtab)
+         then
+           [ fun s => Send PAYD COMPT KSTD envd (StVar KSTD _ screen) Display (SLit _ _ url, tt) ]
+         else
+           []
+       )
+
+    | Quit => fun pl =>
+       let envd := mk_vdesc [] in
+       existT (fun d => hdlr_prog PAYD COMPT KSTD d) envd (
+         let _ := pl in fun st0 =>
+         if fd_eq cfd (shvec_ith (n := projT1 KSTD) _ (projT2 KSTD) (kst _ _ st0) userinput)
+         then
+           [ fun s => Send PAYD COMPT KSTD envd (StVar KSTD _ curtab) Quit tt
+           ; fun s => Send PAYD COMPT KSTD envd (StVar KSTD _ screen) Quit tt
+           ]
+         else
+           []
+       )
+
+    | Some (Some (Some bad)) => fun _ =>
+      match bad with end
+    end (pay PAYD m)
+  ).
+
+Definition main := mk_main (Build_spec NB_MSG PAYD IENVD KSTD COMPT COMPS INIT HANDLERS).
