compiler/dsl/coq/ReflexSSH.v
@@ -1,0 +1,335 @@
+Require Import String.
+
+Require Import Reflex.
+Require Import ReflexBase.
+Require Import ReflexDenoted.
+Require Import ReflexFin.
+Require Import ReflexVec.
+Require Import ReflexHVec.
+
+Open Scope string_scope.
+
+(*
+ This SSH monitor works as follows :
+ 1) the SSH monitor(MON) creates 3 different comps : SYS, SLV, PTY
+ 2) MON waits till SLV sends LoginReq
+
+ == Login Request
+ 1) SLV asks MON to login via LoginReq, 
+ 1-1) if login_cnt =n 3 then send Login_Res(0) back to SLV
+ 1-2) otherwise, login_cnt = login_cnt + 1, then send SysLogReq() 
+ to SYS
+
+ 2) SYS replies to MON with SysLogRes() 
+ if the response is 1 then set login_succeded = 1; and 
+ login_account = $account and MON delivers it to SLV with LogRes  
+
+ == PubKey Request
+ 1) SLV asks MON for the public key via PubKeyReq
+ MON delivers it to SYS via SysPubKeyReq
+  
+ 2) SYS replies to MON with SysPubKeyRes
+ MON delivers it to SLV
+
+ == KeySign Request(str)/IOCTL(fdesc)
+ works in the same as as PubKeyRequest
+
+ == CreatePtyer
+ 1) SLV asks MON for a created PTYER
+ 1-1) if login_succeeded =n 0 then ignore this request completely 
+ and don't send anything back
+
+ 2) MON creates a PTY by sending SysCreatePtyReq()
+ 3) SYS sends back with SysCreatPtyRes(fdesc, fdesc) 
+ (SYS applies ioctl() to the slave fd & it creates a ptyer inside it
+ (Question: there are two options : a. create ptyer inside SYS
+ b. spawns a ptyer as a component from MON. Which one is better?? ) 
+
+ 4) MON replies back to SLV with the two file descriptors
+*)
+
+Definition NB_MSG : nat := 18.
+
+Definition PAYD : vvdesc NB_MSG := mk_vvdesc
+  [ 
+    (* slave <- monitor *)
+    ("LoginReq",   [str_d]);
+    ("LoginResT",   []);
+    ("LoginResF",   []);
+
+    ("PubkeyReq",   []);
+    ("PubkeyRes",   [str_d]);
+
+    ("KeysignReq",   [str_d]);
+    ("KeysignRes",   [str_d]);
+
+    ("CreatePtyerReq",   []);
+    ("CreatePtyerRes",   [fd_d; fd_d]);
+
+    (* monitor <-> system *)
+    ("SLoginReq",   [str_d]);
+    ("SLoginResT",   [str_d]);
+    ("SLoginResF",   []);
+
+    ("SPubkeyReq",   []);
+    ("SPubkeyRes",   [str_d]);
+
+    ("SKeysignReq",   [str_d]);
+    ("SKeysignRes",   [str_d]);
+
+    ("SCreatePtyerReq",   [str_d]);
+    ("SCreatePtyerRes",   [fd_d; fd_d])
+  ].
+ 
+Notation LoginReq :=       (None) (only parsing).
+Notation LoginResT :=      (Some None) (only parsing).
+Notation LoginResF :=      (Some (Some None)) (only parsing).
+      
+Notation PubkeyReq :=      (Some (Some (Some None))) (only parsing).
+Notation PubkeyRes :=      (Some (Some (Some (Some None)))) (only parsing).
+
+Notation KeysignReq :=     (Some (Some (Some (Some (Some None))))) (only parsing).
+Notation KeysignRes :=     (Some (Some (Some (Some (Some (Some None)))))) (only parsing).
+
+Notation CreatePtyerReq := (Some (Some (Some (Some (Some (Some (Some None))))))) (only parsing).
+Notation CreatePtyerRes := (Some (Some (Some (Some (Some (Some (Some (Some None)))))))) (only parsing).
+
+    (* monitor <-> system *)
+Notation SLoginReq :=      (Some (Some (Some (Some (Some (Some (Some (Some (Some None))))))))) (only parsing).
+Notation SLoginResT :=     (Some (Some (Some (Some (Some (Some (Some (Some (Some (Some None)))))))))) (only parsing).
+Notation SLoginResF :=     (Some (Some (Some (Some (Some (Some (Some (Some (Some (Some (Some None))))))))))) (only parsing).
+
+Notation SPubkeyReq :=     (Some (Some (Some (Some (Some (Some (Some (Some (Some (Some (Some (Some None)))))))))))) (only parsing).
+Notation SPubkeyRes :=     (Some (Some (Some (Some (Some (Some (Some (Some (Some (Some (Some (Some (Some None))))))))))))) (only parsing).
+
+Notation SKeysignReq :=    (Some (Some (Some (Some (Some (Some (Some (Some (Some (Some (Some (Some (Some (Some None)))))))))))))) (only parsing).
+Notation SKeysignRes :=    (Some (Some (Some (Some (Some (Some (Some (Some (Some (Some (Some (Some (Some (Some (Some None))))))))))))))) (only parsing).
+
+Notation SCreatePtyerReq := (Some (Some (Some (Some (Some (Some (Some (Some (Some (Some (Some (Some (Some (Some (Some (Some None)))))))))))))))) (only parsing).
+Notation SCreatePtyerRes := (Some (Some (Some (Some (Some (Some (Some (Some (Some (Some (Some (Some (Some (Some (Some (Some (Some None))))))))))))))))) (only parsing).
+
+
+Definition KSTD : vdesc := mk_vdesc
+  [ fd_d (* system *)
+  ; fd_d (* slave *)
+  ; num_d (* authenticated *)
+  ; str_d (* authenticated username *)
+  ].
+
+
+Notation system := (StVar KSTD _ None) (only parsing).
+Notation slave := (StVar KSTD _ (Some None)) (only parsing).
+Notation authenticated := (StVar KSTD _ (Some (Some None))) (only parsing).
+Notation auth_user := (StVar KSTD _ (Some (Some (Some None)))) (only parsing).
+
+Definition IENVD : vdesc := mk_vdesc
+  [ fd_d (* system *)
+  ; fd_d (* slave *)
+  ].
+
+Notation v_system := (None) (only parsing).
+Notation v_slave := (Some None) (only parsing).
+
+Inductive COMPT : Type := System | Slave.
+
+Definition COMPS (t : COMPT) : comp :=
+  match t with
+  | System   => mk_comp "System"   "system"    []
+  | Slave    => mk_comp "Slave"    "slave"     []
+  end.
+
+Definition INIT : init_prog PAYD COMPT KSTD IENVD :=
+  [ fun s => Spawn _ _ _ IENVD System   v_system (Logic.eq_refl _)
+  ; fun s => Spawn _ _ _ IENVD Slave    v_slave (Logic.eq_refl _)
+  ].
+
+
+
+Check @Send.
+(*
+Send
+     : forall (NB_MSG : nat) (VVD : vvdesc NB_MSG) 
+         (COMPT : Type) (KSTD ENVD : vdesc),
+       expr KSTD ENVD fd_d ->
+       forall t : fin NB_MSG,
+       payload_expr KSTD ENVD (lkup_tag VVD t) -> cmd VVD COMPT KSTD ENVD
+*)
+
+Check @StUpd.
+
+
+Check strd_neq_fdd.
+
+Check SLit.
+
+
+
+
+Check KSTD.
+
+Print kst.
+
+Print shvec_ith.
+
+Definition HANDLERS : handlers PAYD COMPT KSTD :=
+  (fun m cfd =>
+    match tag PAYD m as _tm return
+      @sdenote _ SDenoted_vdesc (lkup_tag PAYD _tm) -> _
+    with
+      (* login *)
+
+    | LoginReq => fun pl =>
+       let envd := mk_vdesc [] in
+       existT (fun d => hdlr_prog PAYD COMPT KSTD d) envd (
+         let (loginstr, _) := pl in
+         (fun st0 =>
+            [ fun s => Send PAYD COMPT KSTD envd system SLoginReq (SLit _ _ loginstr, tt)
+            ]
+         )
+       )
+
+    | SLoginResT => fun pl =>
+       let envd := mk_vdesc [] in
+       existT (fun d => hdlr_prog PAYD COMPT KSTD d) envd (
+         let (user, _) := pl in           
+         (fun st0 =>
+            [ 
+              
+              fun s => StUpd PAYD COMPT KSTD envd ((Some (Some (Some None)))) (fun x => strd_neq_fdd x) (SLit _ _ user)
+              ; 
+              fun s => Send PAYD COMPT KSTD envd slave LoginResT tt
+            ]
+         )
+       )
+
+    | SLoginResF => fun pl =>
+       let envd := mk_vdesc [] in
+       existT (fun d => hdlr_prog PAYD COMPT KSTD d) envd (
+         (fun st0 =>
+            [ fun s => Send PAYD COMPT KSTD envd slave LoginResF tt
+            ]
+         )
+       )
+
+       (* pub key request *)
+
+    | PubkeyReq => fun pl =>
+       let envd := mk_vdesc [] in
+       existT (fun d => hdlr_prog PAYD COMPT KSTD d) envd (
+         (fun st0 =>
+            [ fun s => Send PAYD COMPT KSTD envd system SPubkeyReq tt
+            ]
+         )
+       )
+
+    | SPubkeyRes => fun pl =>
+       let envd := mk_vdesc [] in
+       existT (fun d => hdlr_prog PAYD COMPT KSTD d) envd (
+         let (pubkey, _) := pl in
+         (fun st0 =>
+            [ fun s => Send PAYD COMPT KSTD envd system SPubkeyRes (SLit _ _ pubkey, tt)
+            ]
+         )
+       )
+       
+       (* key sign *)
+
+    | KeysignReq => fun pl =>
+       let envd := mk_vdesc [] in
+       existT (fun d => hdlr_prog PAYD COMPT KSTD d) envd (
+         let (keystr, _) := pl in
+         (fun st0 =>
+            [ fun s => Send PAYD COMPT KSTD envd system SKeysignReq (SLit _ _ keystr, tt)
+            ]
+         )
+       )
+
+    | SKeysignRes => fun pl =>
+       let envd := mk_vdesc [] in
+       existT (fun d => hdlr_prog PAYD COMPT KSTD d) envd (
+         let (signedkey, _) := pl in
+         (fun st0 =>
+            [ fun s => Send PAYD COMPT KSTD envd system KeysignRes (SLit _ _ signedkey, tt)
+            ]
+         )
+       )
+
+       (* create pseudo terminal *)
+
+    | CreatePtyerReq => fun pl =>
+       let envd := mk_vdesc [] in
+       existT (fun d => hdlr_prog PAYD COMPT KSTD d) envd (
+         (fun st0 =>
+           if num_eq (shvec_ith _ (projT2 KSTD:svec desc 4) (kst _ _ st0) (Some (Some None)) ) (num_of_nat 0) then []
+             else 
+               [ 
+                 fun s => Send PAYD COMPT KSTD envd system SCreatePtyerReq (auth_user,tt)
+               ]
+         )
+       )
+
+    | SCreatePtyerRes => fun pl =>
+       let envd := mk_vdesc [] in
+       existT (fun d => hdlr_prog PAYD COMPT KSTD d) envd (
+         match pl with 
+           | (fd0, (fd1, _)) =>
+             (fun st0 =>
+               [ fun s => Send PAYD COMPT KSTD envd system CreatePtyerRes (CFd _ _, (CFd _ _, tt))
+               ]
+             )
+         end
+       )
+       
+
+       (* not meant to be received by the kernel *)
+    | LoginResT => fun pl =>
+       let envd := mk_vdesc [] in
+       existT (fun d => hdlr_prog PAYD COMPT KSTD d) envd (
+         (fun st0 => [])
+       )
+    | LoginResF => fun pl =>
+       let envd := mk_vdesc [] in
+       existT (fun d => hdlr_prog PAYD COMPT KSTD d) envd (
+         (fun st0 => [])
+       )
+    | PubkeyRes => fun pl =>
+       let envd := mk_vdesc [] in
+       existT (fun d => hdlr_prog PAYD COMPT KSTD d) envd (
+         (fun st0 => [])
+       )
+    | KeysignRes => fun pl =>
+       let envd := mk_vdesc [] in
+       existT (fun d => hdlr_prog PAYD COMPT KSTD d) envd (
+         (fun st0 => [])
+       )
+    | CreatePtyerRes => fun pl =>
+       let envd := mk_vdesc [] in
+       existT (fun d => hdlr_prog PAYD COMPT KSTD d) envd (
+         (fun st0 => [])
+       )
+    | SLoginReq => fun pl =>
+       let envd := mk_vdesc [] in
+       existT (fun d => hdlr_prog PAYD COMPT KSTD d) envd (
+         (fun st0 => [])
+       )
+    | SPubkeyReq => fun pl =>
+       let envd := mk_vdesc [] in
+       existT (fun d => hdlr_prog PAYD COMPT KSTD d) envd (
+         (fun st0 => [])
+       )
+    | SKeysignReq => fun pl =>
+       let envd := mk_vdesc [] in
+       existT (fun d => hdlr_prog PAYD COMPT KSTD d) envd (
+         (fun st0 => [])
+       )
+    | SCreatePtyerReq => fun pl =>
+       let envd := mk_vdesc [] in
+       existT (fun d => hdlr_prog PAYD COMPT KSTD d) envd (
+         (fun st0 => [])
+       )
+    | (Some (Some (Some (Some (Some (Some (Some (Some (Some (Some (Some (Some (Some (Some (Some (Some (Some (Some bad)))))))))))))))))) => fun _ =>
+      match bad with end
+    end (pay PAYD m)
+  ).
+
+Definition main := mk_main (Build_spec NB_MSG PAYD IENVD KSTD COMPT COMPS INIT HANDLERS).
