compiler/pollang/EchoPolicies.v
@@ -1,17 +1,17 @@
+Require Import Reflex.
 Require Import ReflexEcho.
 Require Import PolLang.
 Require Import ActionMatch.
-Require Import Reflex.
 Require Import Tactics.
 
 Theorem recv_before : forall st tr m,
-  Reach _ _ INIT HANDLERS st -> ktr _ st = inhabits tr ->
-  ImmBefore NB_MSG PAY_DESC
-            (@KORecv NB_MSG PAY_DESC None
-                     (Some (@Build_opt_msg NB_MSG PAY_DESC
+  Reach _ _ COMPS _ _ INIT HANDLERS st -> ktr _ _ st = inhabits tr ->
+  ImmBefore NB_MSG PAYD
+            (@KORecv NB_MSG PAYD None
+                     (Some (@Build_opt_msg NB_MSG PAYD
                                            None (Some m, tt))))
-            (@KOSend NB_MSG PAY_DESC None
-                     (Some (@Build_opt_msg NB_MSG PAY_DESC
+            (@KOSend NB_MSG PAYD None
+                     (Some (@Build_opt_msg NB_MSG PAYD
                                            None (Some m, tt))))
             tr.
 Proof.
@@ -19,13 +19,13 @@ Proof.
 Qed.
 
 Theorem send_after : forall st tr m,
-  Reach _ _ INIT HANDLERS st -> ktr _ st = inhabits tr ->
-  ImmAfter NB_MSG PAY_DESC
-            (@KOSend NB_MSG PAY_DESC None
-                     (Some (@Build_opt_msg NB_MSG PAY_DESC
+  Reach _ _ COMPS _ _ INIT HANDLERS st -> ktr _ _ st = inhabits tr ->
+  ImmAfter NB_MSG PAYD
+            (@KOSend NB_MSG PAYD None
+                     (Some (@Build_opt_msg NB_MSG PAYD
                                            None (Some m, tt))))
-            (@KORecv NB_MSG PAY_DESC None
-                     (Some (@Build_opt_msg NB_MSG PAY_DESC
+            (@KORecv NB_MSG PAYD None
+                     (Some (@Build_opt_msg NB_MSG PAYD
                                            None (Some m, tt))))
             tr.
 Proof.
